step 2

code/ecdsap256/Hacl.Impl.P256.MixedPointAdd.fst
@@ -363,6 +363,118 @@ let point_add_step1 result p q tempBuffer =
   montgomery_multiplication_buffer y3 t2 y3
 
 
+val point_add_step2: result: point -> p: point -> q: pointAffine -> tempBuffer: lbuffer uint64 (size 20) -> Stack unit
+  (requires fun h -> live h result /\ live h p /\ live h q /\ live h tempBuffer /\
+    disjoint p tempBuffer /\ disjoint q tempBuffer /\ eq_or_disjoint result p /\ disjoint result tempBuffer /\ (
+    let t0 = gsub tempBuffer (size 0) (size 4) in 
+    let t1 = gsub tempBuffer (size 4) (size 4) in 
+    let t2 = gsub tempBuffer (size 8) (size 4) in 
+    let t4 = gsub tempBuffer (size 16) (size 4) in  
+
+    let x1 = gsub p (size 0) (size 4) in 
+    let y1 = gsub p (size 4) (size 4) in 
+    let z1 = gsub p (size 8) (size 4) in 
+
+    let x2 = gsub q (size 0) (size 4) in 
+    let y2 = gsub q (size 4) (size 4) in 
+
+    let x3 = gsub result (size 0) (size 4) in 
+    let y3 = gsub result (size 4) (size 4) in 
+    let z3 = gsub result (size 8) (size 4) in 
+
+    as_nat h x1 < prime256 /\
+    as_nat h y1 < prime256 /\
+    as_nat h z1 < prime256 /\
+
+    as_nat h x2 < prime256 /\
+    as_nat h y2 < prime256 /\
+
+    as_nat h x3 < prime256 /\
+    as_nat h y3 < prime256 /\
+    as_nat h z3 < prime256 /\
+
+    as_nat h t0 < prime /\
+    as_nat h t1 < prime /\ 
+    as_nat h t2 < prime /\
+    as_nat h t4 < prime))
+  (ensures fun h0 _ h1 -> modifies (loc result |+| loc tempBuffer) h0 h1 /\ (
+    let z1D = fromDomain_ (as_nat h0 (gsub p (size 8) (size 4))) in 
+
+    let y3D = fromDomain_ (as_nat h0 (gsub result (size 4) (size 4))) in 
+
+    let x3 = gsub result (size 0) (size 4) in 
+    let y3 = gsub result (size 4) (size 4) in 
+    let z3 = gsub result (size 8) (size 4) in 
+
+    let t0 = gsub tempBuffer (size 0) (size 4) in 
+    let t1 = gsub tempBuffer (size 4) (size 4) in 
+    let t2 = gsub tempBuffer (size 8) (size 4) in 
+    let t3 = gsub tempBuffer (size 12) (size 4) in 
+    let t4 = gsub tempBuffer (size 16) (size 4) in 
+
+    let t0D = fromDomain_ (as_nat h0 t0) in 
+    let t4D = fromDomain_ (as_nat h0 t4) in 
+
+    let t1_ = (z1D + z1D) % prime in 
+    let t2_ = (t1_ + z1D) % prime in 
+    let y3_ = (y3D - t2_) % prime in 
+    let y3_ = (y3_ - t0D) % prime in 
+    let t1_ = (y3_ + y3_) % prime in 
+
+    let y3_ = (t1_ + y3_) % prime in 
+    let t1_ = (t0D + t0D) % prime in 
+    let t0_ = (t1_ + t0D) % prime in 
+    let t0_ = (t0_ - t2_) % prime in 
+    let t1_ = (t4D * y3_) % prime in 
+
+    as_nat h1 t0 = toDomain_ t0_ /\
+    as_nat h1 t1 = toDomain_ t1_ /\
+    as_nat h1 t2 = toDomain_ t2_ /\
+    as_nat h1 t3 = as_nat h0 t3 /\
+    as_nat h1 t4 = as_nat h0 t4 /\
+
+    as_nat h1 x3 = as_nat h0 x3 /\
+    as_nat h1 y3 = toDomain_ y3_ /\
+    as_nat h1 z3 = as_nat h0 z3 /\
+
+    as_nat h1 t0 < prime /\
+    as_nat h1 t1 < prime /\
+    as_nat h1 t2 < prime /\
+
+    as_nat h1 y3 < prime))
+
+
+let point_add_step2 result p q tempBuffer = 
+  let x1 = sub p (size 0) (size 4) in 
+  let y1 = sub p (size 4) (size 4) in 
+  let z1 = sub p (size 8) (size 4) in 
+
+  let x2 = sub q (size 0) (size 4) in 
+  let y2 = sub q (size 4) (size 4) in 
+
+  let t0 = sub tempBuffer (size 0) (size 4) in 
+  let t1 = sub tempBuffer (size 4) (size 4) in 
+  let t2 = sub tempBuffer (size 8) (size 4) in 
+  let t3 = sub tempBuffer (size 12) (size 4) in 
+  let t4 = sub tempBuffer (size 16) (size 4) in 
+
+  let x3 = sub result (size 0) (size 4) in 
+  let y3 = sub result (size 4) (size 4) in 
+  let z3 = sub result (size 8) (size 4) in 
+
+  p256_add t1 z1 z1;
+  p256_add t2 t1 z1;
+  p256_sub y3 y3 t2;
+  p256_sub y3 y3 t0;
+  p256_add t1 y3 y3;
+
+  p256_add y3 t1 y3;
+  p256_add t1 t0 t0;
+  p256_add t0 t1 t0;
+  p256_sub t0 t0 t2;
+  montgomery_multiplication_buffer t1 t4 y3
+  
+
 
 (* we except that we already know the q point *)
 val pointAddMixed: result: point -> p: point -> q: pointAffine -> Stack unit 
@@ -375,5 +487,6 @@ let pointAddMixed result p q =
     let tempBuffer = create (size 20) (u64 0) in 
     point_add_step0 result p q tempBuffer;
     point_add_step1 result p q tempBuffer;
+    point_add_step2 result p q tempBuffer;
     copy_point_conditional result q p;
   pop_frame()
